Kami/Ex/Fifo.v
@@ -1,7 +1,7 @@
 Require Import Bool String List.
 Require Import Lib.CommonTactics Lib.ilist Lib.Word Lib.Indexer Lib.StringAsList.
-Require Import Kami.Syntax Kami.ParametricSyntax Kami.Notations Kami.Semantics.
-Require Import Kami.Wf Kami.ParametricEquiv Kami.ParametricWf Kami.Tactics.
+Require Import Kami.Syntax Kami.Notations Kami.Semantics.
+Require Import Kami.Wf Kami.Tactics.
 Require Import FunctionalExtensionality Eqdep Eqdep_dec.
 
 Set Implicit Arguments.
@@ -68,105 +68,10 @@ Section Fifo.
     with Method ^"deq"() : dType := deq
   }.
 
-  (** SinAction version *)
-  Hypothesis HfifoName: index 0 indexSymbol fifoName = None.
-  Lemma fgn:
-    forall s, index 0 indexSymbol s = None -> index 0 indexSymbol (^s) = None.
-  Proof.
-    unfold withPrefix; intros.
-    apply index_not_in; apply index_not_in in H; apply index_not_in in HfifoName.
-    intro Hx; elim H; clear H.
-    apply S_in_app_or in Hx; destruct Hx; auto.
-    apply S_in_app_or in H; destruct H.
-    - inv H; inv H0.
-    - elim HfifoName; auto.
-  Qed.
-
-  Definition enqS {ty} : forall (d: ty dType), SinActionT ty Void := fun d =>
-    (Read isFull <- { ^"full" | fgn "full" eq_refl };
-     Assert !#isFull;
-     Read eltT <- { ^"elt" | fgn "elt" eq_refl };
-     Read enqPT <- { ^"enqP" | fgn "enqP" eq_refl };
-     Read deqPT <- { ^"deqP" | fgn "deqP" eq_refl };
-     Write { ^"elt" | fgn "elt" eq_refl } <- #eltT@[#enqPT <- #d];
-     Write { ^"empty" | fgn "empty" eq_refl } <- $$false;
-     LET next_enqP <- (#enqPT + $1) :: Bit sz;
-     Write { ^"full" | fgn "full" eq_refl } <- (#deqPT == #next_enqP);
-     Write { ^"enqP" | fgn "enqP" eq_refl } <- #next_enqP;
-     Retv)%kami_sin.
-
-  Definition deqS {ty} : SinActionT ty dType :=
-    (Read isEmpty <- { ^"empty" | fgn "empty" eq_refl };
-     Assert !#isEmpty;
-     Read eltT <- { ^"elt" | fgn "elt" eq_refl };
-     Read enqPT <- { ^"enqP" | fgn "enqP" eq_refl };
-     Read deqPT <- { ^"deqP" | fgn "deqP" eq_refl };
-     Write { ^"full" | fgn "full" eq_refl } <- $$false;
-     LET next_deqP <- (#deqPT + $1) :: Bit sz;
-     Write { ^"empty" | fgn "empty" eq_refl } <- (#enqPT == #next_deqP);
-     Write { ^"deqP" | fgn "deqP" eq_refl } <- #next_deqP;
-     Ret #eltT@[#deqPT])%kami_sin.
-
-  Definition firstEltS {ty} : SinActionT ty dType :=
-    (Read isEmpty <- { ^"empty" | fgn "empty" eq_refl };
-     Assert !#isEmpty;
-     Read eltT : Vector dType sz <- { ^"elt" | fgn "elt" eq_refl };
-     Read deqPT <- { ^"deqP" | fgn "deqP" eq_refl };
-     Ret #eltT@[#deqPT])%kami_sin.
-  
-  Definition fifoS := SIN {
-    Register { ^"elt" | fgn "elt" eq_refl } : Vector dType sz <- Default
-    with Register { ^"enqP" | fgn "enqP" eq_refl } : Bit sz <- Default
-    with Register { ^"deqP" | fgn "deqP" eq_refl } : Bit sz <- Default
-    with Register { ^"empty" | fgn "empty" eq_refl } : Bool <- true
-    with Register { ^"full" | fgn "full" eq_refl } : Bool <- Default
-
-    with Method { ^"enq" | fgn "enq" eq_refl }(d : dType) : Void := (enqS d)
-    with Method { ^"deq" | fgn "deq" eq_refl }() : dType := deqS
-    with Method { ^"firstElt" | fgn "firstElt" eq_refl }() : dType := firstEltS
-  }.
-
-  Definition fifoM := META {
-    Register { ^"elt" | fgn "elt" eq_refl } : Vector dType sz <- Default
-    with Register { ^"enqP" | fgn "enqP" eq_refl } : Bit sz <- Default
-    with Register { ^"deqP" | fgn "deqP" eq_refl } : Bit sz <- Default
-    with Register { ^"empty" | fgn "empty" eq_refl } : Bool <- true
-    with Register { ^"full" | fgn "full" eq_refl } : Bool <- Default
-
-    with Method { ^"enq" | fgn "enq" eq_refl }(d : dType) : Void := (enqS d)
-    with Method { ^"deq" | fgn "deq" eq_refl }() : dType := deqS
-    with Method { ^"firstElt" | fgn "firstElt" eq_refl }() : dType := firstEltS
-  }.
-
-  Definition simpleFifoS := SIN {
-    Register { ^"elt" | fgn "elt" eq_refl } : Vector dType sz <- Default
-    with Register { ^"enqP" | fgn "enqP" eq_refl } : Bit sz <- Default
-    with Register { ^"deqP" | fgn "deqP" eq_refl } : Bit sz <- Default
-    with Register { ^"empty" | fgn "empty" eq_refl } : Bool <- true
-    with Register { ^"full" | fgn "full" eq_refl } : Bool <- Default
-
-    with Method { ^"enq" | fgn "enq" eq_refl }(d : dType) : Void := (enqS d)
-    with Method { ^"deq" | fgn "deq" eq_refl }() : dType := deqS
-  }.
-
-  Definition simpleFifoM := META {
-    Register { ^"elt" | fgn "elt" eq_refl } : Vector dType sz <- Default
-    with Register { ^"enqP" | fgn "enqP" eq_refl } : Bit sz <- Default
-    with Register { ^"deqP" | fgn "deqP" eq_refl } : Bit sz <- Default
-    with Register { ^"empty" | fgn "empty" eq_refl } : Bool <- true
-    with Register { ^"full" | fgn "full" eq_refl } : Bool <- Default
-
-    with Method { ^"enq" | fgn "enq" eq_refl }(d : dType) : Void := (enqS d)
-    with Method { ^"deq" | fgn "deq" eq_refl }() : dType := deqS
-  }.
-
 End Fifo.
 
 Hint Unfold fifo simpleFifo : ModuleDefs.
 Hint Unfold enq deq firstElt : MethDefs.
-
-Hint Unfold fifoS simpleFifoS : ModuleDefs.
-Hint Unfold enqS deqS firstEltS : MethDefs.
 
 Section Facts.
   Variable fifoName: string.
@@ -174,22 +79,6 @@ Section Facts.
   Variable dType: Kind.
 
   Hypothesis HfifoName: index 0 indexSymbol fifoName = None.
-
-  Lemma fifo_fifoM:
-    fifo fifoName sz dType = modFromMeta (fifoM fifoName sz dType HfifoName).
-  Proof. reflexivity. Qed.
-
-  Lemma fifo_fifoS:
-    fifo fifoName sz dType = getModFromSin (fifoS fifoName sz dType HfifoName).
-  Proof. reflexivity. Qed.
-
-  Lemma simpleFifo_simpleFifoM:
-    simpleFifo fifoName sz dType = modFromMeta (simpleFifoM fifoName sz dType HfifoName).
-  Proof. reflexivity. Qed.
-
-  Lemma simpleFifo_simpleFifoS:
-    simpleFifo fifoName sz dType = getModFromSin (simpleFifoS fifoName sz dType HfifoName).
-  Proof. reflexivity. Qed.
 
   Lemma fifo_ModEquiv:
     ModPhoasWf (fifo fifoName sz dType).
@@ -211,63 +100,8 @@ Section Facts.
   Proof. kvr. Qed.
   Hint Resolve simpleFifo_ValidRegs.
 
-  Variable n: nat.
-
-  Lemma fifoSS_ModEquiv:
-    ModPhoasWf (getModFromSin (fifoS fifoName sz dType HfifoName)).
-  Proof. rewrite <-fifo_fifoS; kequiv. Qed.
-
-  Lemma fifoS_ModEquiv:
-    MetaModPhoasWf (getMetaFromSinNat n (fifoS fifoName sz dType HfifoName)).
-  Proof. kequiv. Qed.
-
-  Lemma fifoM_ModEquiv:
-    MetaModPhoasWf (fifoM fifoName sz dType HfifoName).
-  Proof. kequiv. Qed.
-
-  Lemma simpleFifoSS_ModEquiv:
-    ModPhoasWf (getModFromSin (simpleFifoS fifoName sz dType HfifoName)).
-  Proof. rewrite <-simpleFifo_simpleFifoS; kequiv. Qed.
-
-  Lemma simpleFifoS_ModEquiv:
-    MetaModPhoasWf (getMetaFromSinNat n (simpleFifoS fifoName sz dType HfifoName)).
-  Proof. kequiv. Qed.
-
-  Lemma simpleFifoM_ModEquiv:
-    MetaModPhoasWf (simpleFifoM fifoName sz dType HfifoName).
-  Proof. kequiv. Qed.
-
-  Lemma fifoSS_ValidRegs:
-    ModRegsWf (getModFromSin (fifoS fifoName sz dType HfifoName)).
-  Proof. rewrite <-fifo_fifoS; kvr. Qed.
-  
-  Lemma fifoS_ValidRegs:
-    MetaModRegsWf (getMetaFromSinNat n (fifoS fifoName sz dType HfifoName)).
-  Proof. kvr. Qed.
-
-  Lemma fifoM_ValidRegs:
-    MetaModRegsWf (fifoM fifoName sz dType HfifoName).
-  Proof. kvr. Qed.
-
-  Lemma simpleFifoSS_ValidRegs:
-    ModRegsWf (getModFromSin (simpleFifoS fifoName sz dType HfifoName)).
-  Proof. rewrite <-simpleFifo_simpleFifoS; kvr. Qed.
-
-  Lemma simpleFifoS_ValidRegs:
-    MetaModRegsWf (getMetaFromSinNat n (simpleFifoS fifoName sz dType HfifoName)).
-  Proof. kvr. Qed.
-
-  Lemma simpleFifoM_ValidRegs:
-    MetaModRegsWf (simpleFifoM fifoName sz dType HfifoName).
-  Proof. kvr. Qed.
-
 End Facts.
 
-Hint Resolve fifo_ModEquiv simpleFifo_ModEquiv
-     fifoS_ModEquiv fifoSS_ModEquiv fifoM_ModEquiv
-     simpleFifoS_ModEquiv simpleFifoSS_ModEquiv simpleFifoM_ModEquiv.
-     
-Hint Resolve fifo_ValidRegs simpleFifo_ValidRegs
-     fifoS_ValidRegs fifoSS_ValidRegs fifoM_ValidRegs
-     simpleFifoS_ValidRegs simpleFifoSS_ValidRegs simpleFifoM_ValidRegs.
+Hint Resolve fifo_ModEquiv simpleFifo_ModEquiv.
+Hint Resolve fifo_ValidRegs simpleFifo_ValidRegs.
 
