Kami/InlineFacts.v
@@ -441,8 +441,8 @@ Proof.
   simpl.
 
   clear; induction m; unfold getDefs in *; simpl in *.
-  - induction read; simpl; auto.
-    unfold namesOf in *; inversion IHread; rewrite map_map in *; repeat f_equal; auto.
+  - clear; induction (pm_methods prim); [auto|].
+    simpl; f_equal; auto.
   - clear; induction dms; [auto|].
     simpl; f_equal; auto.
   - apply inlineDmToDms_names.
@@ -714,14 +714,15 @@ Proof.
   destruct m; intros; simpl in *.
   - unfold inlineDmToMod.
     try destruct (getAttribute _ _);
-      try (reflexivity; fail).
-    induction read; simpl; auto.
-    inversion IHread; unfold namesOf in *; rewrite? map_map in *; repeat f_equal; auto.
+    try (reflexivity; fail).
+    simpl; clear.
+    induction (pm_methods prim); auto.
+    simpl; f_equal; auto.
+
   - unfold inlineDmToMod.
     try destruct (getAttribute _ _);
     try (reflexivity; fail).
     simpl; clear.
-
     induction dms; auto.
     simpl; f_equal; auto.
 
