Kami/Kami.v
@@ -3,7 +3,6 @@ Require Export Bool String List.
 Require Export Lib.FMap Lib.Word Lib.CommonTactics Lib.Indexer.
 
 Require Export Kami.Syntax Kami.Semantics Kami.Wf Kami.Notations.
-Require Export Kami.ParametricSyntax Kami.ParametricEquiv Kami.ParametricInline Kami.ParametricInlineLtac Kami.ParametricWf Kami.PartialInlineFacts.
 Require Export Kami.RefinementFacts Kami.Decomposition.
-Require Export Kami.Inline Kami.InlineFacts.
+Require Export Kami.Inline Kami.InlineFacts Kami.PartialInlineFacts.
 Require Export Kami.Tactics.
