Kami/Synthesize.v
@@ -8,69 +8,73 @@ Definition tyS: Kind -> Type := fun _ => nat.
 Definition ExprS := Expr tyS.
 
 Inductive ActionS (lretT: Kind) : Type :=
-  | MCallS (meth: string) s:
-      ExprS (SyntaxKind (arg s)) ->
+| MCallS (meth: string) s:
+    ExprS (SyntaxKind (arg s)) ->
+    nat ->
+    ActionS lretT ->
+    ActionS lretT
+| LetS_ lretT': ExprS lretT' -> nat -> ActionS lretT -> ActionS lretT
+| ReadNondetS:
+    nat -> ActionS lretT -> ActionS lretT
+| ReadRegS (r: string):
+    nat -> ActionS lretT -> ActionS lretT
+| WriteRegS (r: string) k:
+    ExprS k -> ActionS lretT -> ActionS lretT
+| IfElseS: ExprS (SyntaxKind Bool) -> forall k,
+      ActionS k ->
+      ActionS k ->
       nat ->
       ActionS lretT ->
       ActionS lretT
-  | LetS_ lretT': ExprS lretT' -> nat -> ActionS lretT -> ActionS lretT
-  | ReadNondetS:
-      nat -> ActionS lretT -> ActionS lretT
-  | ReadRegS (r: string):
-      nat -> ActionS lretT -> ActionS lretT
-  | WriteRegS (r: string) k:
-      ExprS k -> ActionS lretT -> ActionS lretT
-  | IfElseS: ExprS (SyntaxKind Bool) -> forall k,
-                                        ActionS k ->
-                                        ActionS k ->
-                                        nat ->
-                                        ActionS lretT ->
-                                        ActionS lretT
-  | AssertS_: ExprS (SyntaxKind Bool) -> ActionS lretT -> ActionS lretT
-  | ReturnS: ExprS (SyntaxKind lretT) -> ActionS lretT.
+| AssertS_: ExprS (SyntaxKind Bool) -> ActionS lretT -> ActionS lretT
+| ReturnS: ExprS (SyntaxKind lretT) -> ActionS lretT.
 
-Fixpoint getActionS (n: nat) lret (a: ActionT tyS lret) {struct a}: (nat * ActionS lret) :=
+Fixpoint getActionS (n: nat) lret (a: ActionT tyS lret) {struct a}
+  : (nat * ActionS lret) :=
   match a with
-    | MCall meth s e c =>
-      let (m, a') := @getActionS (S n) _ (c n) in
-      (m, MCallS meth s e n a')
-    | Let_ lret' e cn => match lret' return (nat * ActionS lret) -> nat * ActionS lret with
-                           | SyntaxKind k => fun v => (fst v,
-                                                       LetS_ e n (snd v))
-                           | NativeKind _ _ => fun _ => (n, ReturnS (Const tyS Default))
-                         end (@getActionS (S n) _ (cn match lret' with
-                                                        | SyntaxKind k => n
-                                                        | NativeKind t c => c
-                                                      end))
-    | ReadNondet k cn => match k return (nat * ActionS lret) -> nat * ActionS lret with
-                         | SyntaxKind k => fun v => (fst v,
-                                                     ReadNondetS n (snd v))
-                         | NativeKind _ _ => fun _ => (n, ReturnS (Const tyS Default))
-                         end (@getActionS (S n) _ (cn match k with
-                                                      | SyntaxKind _ => n
-                                                      | NativeKind t c => c
-                                                      end))
-    | ReadReg r k cn => match k return (nat * ActionS lret) -> nat * ActionS lret with
-                          | SyntaxKind k => fun v => (fst v,
-                                                      ReadRegS r n (snd v))
-                          | NativeKind _ _ => fun _ => (n, ReturnS (Const tyS Default))
-                        end (@getActionS (S n) _ (cn match k with
-                                                       | SyntaxKind _ => n
-                                                       | NativeKind t c => c
-                                                     end))
-    | WriteReg r _ e c =>
-      let (m, a') := @getActionS n _ c in
-      (m, WriteRegS r e a')
-    | IfElse e _ ta fa c =>
-      let (tm, ta') := @getActionS n _ ta in
-      let (fm, fa') := @getActionS tm _ fa in
-      let (m, a') := @getActionS (S fm) _ (c fm) in
-      (m, IfElseS e ta' fa' fm a')
-    | Assert_ e c =>
-      let (m, a') := @getActionS n _ c in
-      (m, AssertS_ e a')
-    | Displ ls c => @getActionS n _ c
-    | Return e => (n, ReturnS e)
+  | MCall meth s e c =>
+    let (m, a') := @getActionS (S n) _ (c n) in
+    (m, MCallS meth s e n a')
+  | Let_ lret' e cn =>
+    match lret' return (nat * ActionS lret) -> nat * ActionS lret with
+    | SyntaxKind k => fun v => (fst v,
+                                LetS_ e n (snd v))
+    | NativeKind _ _ => fun _ => (n, ReturnS (Const tyS Default))
+    end (@getActionS (S n) _ (cn match lret' with
+                                 | SyntaxKind k => n
+                                 | NativeKind t c => c
+                                 end))
+  | ReadNondet k cn =>
+    match k return (nat * ActionS lret) -> nat * ActionS lret with
+    | SyntaxKind k => fun v => (fst v,
+                                ReadNondetS n (snd v))
+    | NativeKind _ _ => fun _ => (n, ReturnS (Const tyS Default))
+    end (@getActionS (S n) _ (cn match k with
+                                 | SyntaxKind _ => n
+                                 | NativeKind t c => c
+                                 end))
+  | ReadReg r k cn =>
+    match k return (nat * ActionS lret) -> nat * ActionS lret with
+    | SyntaxKind k => fun v => (fst v,
+                                ReadRegS r n (snd v))
+    | NativeKind _ _ => fun _ => (n, ReturnS (Const tyS Default))
+    end (@getActionS (S n) _ (cn match k with
+                                 | SyntaxKind _ => n
+                                 | NativeKind t c => c
+                                 end))
+  | WriteReg r _ e c =>
+    let (m, a') := @getActionS n _ c in
+    (m, WriteRegS r e a')
+  | IfElse e _ ta fa c =>
+    let (tm, ta') := @getActionS n _ ta in
+    let (fm, fa') := @getActionS tm _ fa in
+    let (m, a') := @getActionS (S fm) _ (c fm) in
+    (m, IfElseS e ta' fa' fm a')
+  | Assert_ e c =>
+    let (m, a') := @getActionS n _ c in
+    (m, AssertS_ e a')
+  | Displ ls c => @getActionS n _ c
+  | Return e => (n, ReturnS e)
   end.
   
 Definition MethodTS sig := ActionS (ret sig).
@@ -78,10 +82,10 @@ Definition MethodTS sig := ActionS (ret sig).
 Definition DefMethTS := Attribute (sigT MethodTS).
 
 Inductive ModulesS: Type :=
-| RegFileS (dataArray: string) (read: list string) (write: string) (IdxBits: nat) (Data: Kind) (init: ConstT (Vector Data IdxBits))
+| PrimModS (primModName: string) (ifc: list (Attribute SignatureT))
 | ModS (regs: list RegInitT)
-      (rules: list (Attribute (ActionS Void)))
-      (dms: list DefMethTS):
+       (rules: list (Attribute (ActionS Void)))
+       (dms: list DefMethTS):
     ModulesS
 | ConcatModsS (m1 m2: ModulesS):
     ModulesS.
@@ -91,16 +95,20 @@ Definition getMethS (x: sigT MethodT): sigT MethodTS :=
     | existT arg meth => existT _ arg (snd (getActionS 1 (meth tyS 0)))
   end.
 
-Fixpoint getModuleS (m: Modules): ModulesS.
-Proof.
-  refine (match m with
-            | RegFile dataArray read write IdxBits Data init => RegFileS dataArray read write init
-            | Mod regs rules dms =>
-              ModS regs (map (fun a => {| attrName := attrName a;
-                                          attrType := snd (getActionS 0 _) |} ) rules)
-                   (map (fun a => {| attrName := attrName a;
-                                     attrType := getMethS (attrType a) |}) dms)
-            | ConcatMod m1 m2 => ConcatModsS (getModuleS m1) (getModuleS m2)
-          end).
-  exact (attrType a tyS).
-Defined.
+Fixpoint getModuleS (m: Modules): ModulesS :=
+  match m with
+  | PrimMod prim =>
+    PrimModS (pm_name prim)
+             (map (fun dm => (attrName dm :: projT1 (attrType dm))%struct) 
+                  (pm_methods prim))
+  | Mod regs rules dms =>
+    ModS regs
+         (map
+            (fun a: Attribute (Action Void) =>
+               (attrName a :: snd (getActionS 0 (attrType a tyS)))%struct)
+            rules)
+         (map (fun a => (attrName a :: getMethS (attrType a))%struct) dms)
+  | ConcatMod m1 m2 =>
+    ConcatModsS (getModuleS m1) (getModuleS m2)
+  end.
+
